Ch5.thy
@@ -1,0 +1,30 @@
+theory Ch5
+  imports Main
+begin
+
+(*
+
+see of and OF 4.4.4
+
+f.simps refers to the whole list of recursion equations defining
+f. Individual facts can be selected by writing f.simps(2), whole sublists by
+writing f.simps(2−4).
+
+*)
+
+lemma "\<not> surj (f :: 'a \<Rightarrow> 'a set )"
+proof
+assume 0: "surj f"
+from 0 have 1: "\<forall> A. \<exists> a. A = f a" by(simp add: surj_def)
+from 1 have 2: "\<exists> a. {x . x \<notin> f x } = f a" by blast
+from 2 show "False" by blast
+qed
+
+lemma "\<not> surj (f :: 'a \<Rightarrow> 'a set )"
+proof
+assume "surj f"
+  hence "\<exists> a. {x . x \<notin> f x } = f a" by(auto simp: surj_def)
+  thus "False" by blast
+qed
+
+end
